\documentclass[fleqn]{article}
\usepackage[spanish]{babel}
\usepackage{amsmath, amssymb, amsfonts}
\usepackage{parskip}
\usepackage[scr]{rsfso}

\begin{document}
    31. $ \dfrac{\mathrm{d} y}{\mathrm{d} t} - y = 1 $; $ y(0) = 0 $

    \textbf{Solución.}

    $ \mathscr{L} \left\lbrace \dfrac{\mathrm{d} y}{\mathrm{d} t} - y \right\rbrace = \mathscr{L} \lbrace 1 \rbrace $

    $ \Longrightarrow s Y(s) - y(0) - Y(s) = \dfrac{1}{s} $

    $ \Longrightarrow Y(s)(s - 1) = \dfrac{1}{s} $

    $ \Longrightarrow Y(s) = \dfrac{1}{s(s - 1)} $

    Sea $ \dfrac{1}{s(s - 1)} = \dfrac{A}{s} + \dfrac{B}{s - 1} $

    $ \Longrightarrow 1 = A(s-1) + Bs = s(A + B) - A $

    $ \Longrightarrow A + B = 0 $ y $ -A = 1 $

    $ \Longrightarrow A = -1 $ y $ B = 1 $

    Así, $ Y(s) = -\dfrac{1}{s} + \dfrac{1}{s - 1} $.

    Aplicando Transformada Inversa de Laplace

    $ \mathscr{L}^{-1} \lbrace Y(s) \rbrace = \mathscr{L}^{-1} \left\lbrace -\dfrac{1}{s} + \dfrac{1}{s - 1} \right\rbrace $

    $ \therefore y(t) = -1 + e^t $

    32. $ 2 \, \dfrac{\mathrm{d} y}{\mathrm{d} t} + y = 0 $; $ y(0) = -3 $

    \textbf{Solución.}

    $ \mathscr{L} \left\lbrace 2 \, \dfrac{\mathrm{d} y}{\mathrm{d} t} + y \right\rbrace = \mathscr{L} \lbrace 0 \rbrace $

    $ \Longrightarrow 2s Y(s) - 2y(0) + Y(s) = 0 $

    $ \Longrightarrow Y(s)(2s + 1) = -6 $

    $ \Longrightarrow Y(s) = \dfrac{-6}{2s + 1} $

    Aplicando Transformada Inversa de Laplace

    $ \mathscr{L}^{-1} \lbrace Y(s) \rbrace = \mathscr{L}^{-1} \left\lbrace \dfrac{-6}{2s + 1} \right\rbrace = \mathscr{L}^{-1} \left\lbrace \dfrac{-3}{s + \frac{1}{2}} \right\rbrace $

    $ \therefore y(t) = -3 e^{- \frac{t}{2}} $

    33. $ y' + 6y = e^{4t} $; $ y(0) = 2 $

    \textbf{Solución.}

    $ \mathscr{L} \left\lbrace y' + 6y \right\rbrace = \mathscr{L} \lbrace e^{4t} \rbrace $

    $ \Longrightarrow s Y(s) - y(0) + 6Y(s) = \dfrac{1}{s - 4} $

    $ \Longrightarrow Y(s)(s + 6) = \dfrac{1}{s - 4} + 2 $

    $ \Longrightarrow Y(s) = \dfrac{2s - 7}{(s - 4)(s + 6)} $

    Sea $ \dfrac{2s - 7}{(s - 4)(s + 6)} = \dfrac{A}{s - 4} + \dfrac{B}{s + 6} $

    $ \Longrightarrow 2s - 7 = A(s+6) + B(s-4) = s(A + B) + 6A - 4B $
    \begin{align}
        \Longrightarrow &A + B = 2 \label{eq:1} \\
        &6A - 4B = -7 \label{eq:2}
    \end{align}
    De (\ref{eq:1}): $ A = 2 - B $. Sustituyendo en (\ref{eq:2}) se tiene que $ -7 = 6(2 - B) - 4B = 12 - 6B - 4B = 12 - 10B \Longrightarrow B = \dfrac{19}{10} $. Así, $ A = 2 - \dfrac{19}{10} = \dfrac{1}{10} $.

    De esta manera, $ Y(s) = \dfrac{\frac{1}{10}}{s - 4} + \dfrac{\frac{19}{10}}{s + 6} $.

    Aplicando Transformada Inversa de Laplace

    $ \mathscr{L}^{-1} \lbrace Y(s) \rbrace = \mathscr{L}^{-1} \left\lbrace \dfrac{\frac{1}{10}}{s - 4} + \dfrac{\frac{19}{10}}{s + 6} \right\rbrace $ 

    $ \therefore y(t) = \dfrac{e^{4t}}{10} + \dfrac{19 e^{-6t}}{10} $

    34. $ y' - y = 2 \cos (5t) $; $ y(0) = 0 $
    
    \textbf{Solución.}

    $ \mathscr{L} \left\lbrace y' - y \right\rbrace = \mathscr{L} \lbrace 2 \cos (5t) \rbrace $

    $ \Longrightarrow s Y(s) - y(0) - Y(s) = \dfrac{2s}{s^2 + 25} $

    $ \Longrightarrow Y(s)(s - 1) = \dfrac{2s}{s^2 + 25} $

    $ \Longrightarrow Y(s) = \dfrac{2s}{(s - 1)(s^2 + 25)} $

    Sea $ \dfrac{2s}{(s^2 + 25)} = \dfrac{A}{s - 1} + \dfrac{Bs + C}{s^2 + 25} $

    $ \Longrightarrow 2s = A(s^2 + 25) + (Bs + C)(s - 1) = s^2(A + B) + s(-B + C) + 25A - C $
    \begin{align}
        \Longrightarrow &A + B = 0 \label{eq:3} \\
        & -B + C = 2 \label{eq:4} \\
        & 25A - C = 0 \label{eq:5}
    \end{align}
    Sumando (\ref{eq:4}) y (\ref{eq:5}): 25A - B = 2. De (\ref{eq:3}): $ A = -B $. Así, $ -25B - B = -26B = 2 \Longrightarrow B = - \dfrac{1}{13} $. Luego, $ A = \dfrac{1}{13} $ y $ C = \dfrac{25}{13} $.

    Por lo que, $ Y(s) = \dfrac{\frac{1}{13}}{s - 1} - \dfrac{\frac{1}{13} \, s - \frac{25}{13}}{s^2 + 25} $

    Aplicando Transformada Inversa de Laplace

    $ \mathscr{L}^{-1} \lbrace Y(s) \rbrace = \mathscr{L}^{-1} \left\lbrace \dfrac{\frac{1}{13}}{s - 1} - \dfrac{\frac{1}{13} \, s - \frac{25}{13}}{s^2 + 25} \right\rbrace $ 

    $ \therefore y(t) = \dfrac{e^t}{13} - \dfrac{\cos (5t)}{13}  + \dfrac{5 \sen (5t)}{13} $

\end{document}