documentclass{article}
\begin{document}
      5. $ \frac{dN}{dt}+N=Nte^{t+2} $
      $ \Longrightarrow \frac{dN}{dt}=Nte^{t+2}-N $
      $ \Longrightarrow \frac{dN}{dt}=N(te^{t+2}-1) $
      Sea $ N \neq 0 $, entonces
      $ frac{1}{N} \cdot \frac{dN}{dt}=te^{t+2}-1 $
      $ \Longrightarrow \int frac{1}{N} \mathrm{d}N = \int (te^{t+2}-1) \mathrm{d}t $
      $ \Longrightarrow \ln \| N = \int te^{t+2} \mathrm{d}t - \int 1 \mathrm{d}t $
      Sea $ u=t $ y $ \mathrm{d}v = e^{t+2} $ entonces $ \mathrm{d}u = \mathrm{d}t $ y $ v = e^{t+2} $}. Así,
      $ \ln \| N = te^{t+2} - \int e^{t+2}\mathrm{d}t - t $
      $ \Longrightarrow \ln \| N = te^{t+2} - e^{t+2} - t + c $
      $ \Longrightarrow N = e^c \ cdot e^{te^{t+2} - e^{t+2} - t} $
      Como no existe algún $ c $ que satisface que $ N = 0 $, entonces $ N = e^c \ cdot e^{te^{t+2} - e^{t+2} - t} $ es solución explícita de la E.D.
\end{document}
